Add `States.EQ`

PGCL/IdleInduction.lean
@@ -13,10 +13,12 @@ theorem wlp_apply_eq_wlp''_apply {C : pGCL Γ} :
     wlp[O]⟦@C⟧ X σ = wlp''[O]⟦@C⟧ X σ := by
   simp [wlp'']
 
+def States.EQ (V : Set 𝒱) (σ₀ : States Γ) : Set (States Γ) := {σ | ∀ v ∈ V, σ v = σ₀ v}
+
 /-- An _Idle invariant_ is _Park invariant_ that holds for states with a set of fixed variables. -/
 def IdleInvariant (g : 𝔼[Γ, ENNReal] →o 𝔼[Γ, ENNReal]) (b : BExpr Γ) (φ : 𝔼[Γ, ENNReal])
-    (I : 𝔼[Γ, ENNReal]) (S : Set 𝒱) (σ₀ : States Γ) : Prop :=
-  ∀ σ, (∀ v ∈ S, σ v = σ₀ v) → Ψ[g] b φ I σ ≤ I σ
+    (I : 𝔼[Γ, ENNReal]) (V : Set 𝒱) (σ₀ : States Γ) : Prop :=
+  ∀ σ ∈ σ₀.EQ V, Ψ[g] b φ I σ ≤ I σ
 
 /-- _Idle induction_ is _Park induction_, but the engine is running (i.e. an initial state is
 given), and as a consequence only states that vary over the modified variables need to be
@@ -33,13 +35,13 @@ theorem IdleInduction {b : BExpr Γ} {C : pGCL Γ} {φ : 𝔼[Γ, ENNReal]} {I :
   simp [IdleInvariant, Ψ] at h
   rw [← C.wp_fix I C.modsᶜ (by simp)]
   convert h (σ₀.cofix σ') ?_
-  simp +contextual
+  simp +contextual [States.EQ]
 
 /-- An _Idle coinvariant_ is _Park coinvariant_ that holds for states with a set of fixed variables.
 -/
 def IdleCoinvariant (g : 𝔼[Γ, ENNReal] →o 𝔼[Γ, ENNReal]) (b : BExpr Γ) (φ : 𝔼[Γ, ENNReal])
-    (I : 𝔼[Γ, ENNReal]) (S : Set 𝒱) (σ₀ : States Γ) : Prop :=
-  ∀ σ, (∀ v ∈ S, σ v = σ₀ v) → I σ ≤ Ψ[g] b φ I σ
+    (I : 𝔼[Γ, ENNReal]) (V : Set 𝒱) (σ₀ : States Γ) : Prop :=
+  ∀ σ ∈ σ₀.EQ V, I σ ≤ Ψ[g] b φ I σ
 
 /-- _Idle coinduction_ is _Park coinduction_, but the engine is running (i.e. an initial state is
 given), and as a consequence only states that vary over the modified variables need to be
@@ -62,12 +64,12 @@ theorem IdleCoinduction {b : BExpr Γ} {C : pGCL Γ} {φ : 𝔼[Γ, ENNReal]} {I
   convert h (σ₀.cofix σ') ?_
   · simp [Iverson.iver]; split <;> simp_all [wlp'', ProbExp.ofExp]
     apply hφ
-  · simp +contextual
+  · simp +contextual [States.EQ]
 
 /-- A _Idle k-invariant_. -/
 def IdleKInvariant (g : 𝔼[Γ, ENNReal] →o 𝔼[Γ, ENNReal]) (b : BExpr Γ) (φ : 𝔼[Γ, ENNReal]) (k : ℕ)
-    (I : 𝔼[Γ, ENNReal]) (S : Set 𝒱) (σ₀ : States Γ) : Prop :=
-    ∀ σ, (∀ v ∈ S, σ v = σ₀ v) → (Ψ[g] b φ) ((Ψ[g] b φ · ⊓ I)^[k] I) σ ≤ I σ
+    (I : 𝔼[Γ, ENNReal]) (V : Set 𝒱) (σ₀ : States Γ) : Prop :=
+    ∀ σ ∈ σ₀.EQ V, (Ψ[g] b φ) ((Ψ[g] b φ · ⊓ I)^[k] I) σ ≤ I σ
 
 /-- _Idle k-induction_. -/
 theorem IdleKInduction {b : BExpr Γ} {C : pGCL Γ} {φ : 𝔼[Γ, ENNReal]} {I : 𝔼[Γ, ENNReal]} (k : ℕ)
@@ -99,12 +101,12 @@ theorem IdleKInduction {b : BExpr Γ} {C : pGCL Γ} {φ : 𝔼[Γ, ENNReal]} {I 
   simp [this]
   rw [← wp_fix _ _ _ (by simp)]
   convert h (σ₀.cofix σ') ?_
-  · simp +contextual
+  · simp +contextual [States.EQ]
 
 /-- A _Idle k-coinvariant_. -/
 def IdleKCoinvariant (g : ProbExp Γ →o ProbExp Γ) (b : BExpr Γ) (φ : ProbExp Γ) (k : ℕ)
-    (I : ProbExp Γ) (S : Set 𝒱) (σ₀ : States Γ) : Prop :=
-    ∀ σ, (∀ v ∈ S, σ v = σ₀ v) → I σ ≤ (pΨ[g] b φ) ((pΨ[g] b φ · ⊔ I)^[k] I) σ
+    (I : ProbExp Γ) (V : Set 𝒱) (σ₀ : States Γ) : Prop :=
+    ∀ σ ∈ σ₀.EQ V, I σ ≤ (pΨ[g] b φ) ((pΨ[g] b φ · ⊔ I)^[k] I) σ
 
 /-- _Idle k-coinduction_. -/
 theorem IdleKCoinduction {b : BExpr Γ} {C : pGCL Γ} {φ : ProbExp Γ} {I : ProbExp Γ} (k : ℕ)
@@ -139,12 +141,12 @@ theorem IdleKCoinduction {b : BExpr Γ} {C : pGCL Γ} {φ : ProbExp Γ} {I : Pro
   simp [this]
   rw [← wlp_fix _ _ _ (by simp)]
   convert h (σ₀.cofix σ') ?_
-  · simp +contextual
+  · simp +contextual [States.EQ]
 
 /-- A _Idle k-coinvariant_. -/
 def IdleKCoinvariant'' (g : 𝔼[Γ, ENNReal] →o 𝔼[Γ, ENNReal]) (b : BExpr Γ) (φ : 𝔼[Γ, ENNReal])
-    (k : ℕ) (I : 𝔼[Γ, ENNReal]) (S : Set 𝒱) (σ₀ : States Γ) : Prop :=
-    ∀ σ, (∀ v ∈ S, σ v = σ₀ v) → I σ ≤ (Ψ[g] b φ) ((Ψ[g] b φ · ⊔ I)^[k] I) σ
+    (k : ℕ) (I : 𝔼[Γ, ENNReal]) (V : Set 𝒱) (σ₀ : States Γ) : Prop :=
+    ∀ σ ∈ σ₀.EQ V, I σ ≤ (Ψ[g] b φ) ((Ψ[g] b φ · ⊔ I)^[k] I) σ
 
 def IdleKCoinvariant''.toIdleKCoinvariant {C : pGCL Γ}
     (h : IdleKCoinvariant'' wlp''[O]⟦@C⟧ b φ k I C.modsᶜ σ₀) (hI : I ≤ 1) (hφ : φ ≤ 1) :
